theories/rules/rules_Get.v
@@ -17,26 +17,13 @@ Section cap_lang_rules.
   Implicit Types reg : gmap RegName Word.
   Implicit Types ms : gmap Addr Word.
 
-  (* TODO: move to stdpp *)
-  Tactic Notation "destruct_or" ident(H) :=
-  match type of H with
-  | _ ∨ _ => destruct H as [H|H]
-  | Is_true (_ || _) => apply orb_True in H; destruct H as [H|H]
-  end.
-  Tactic Notation "destruct_or" "?" ident(H) := repeat (destruct_or H).
-  Tactic Notation "destruct_or" "!" ident(H) := hnf in H; destruct_or H; destruct_or? H.
-
-
-  Definition denote (i: instr) (c: Cap): Z :=
-    match c with
-    | (p, b, e, a) =>
-      match i with
-      | GetP _ _ => encodePerm p
-      | GetB _ _ => b
-      | GetE _ _ => e
-      | GetA _ _ => a
-      | _ => 0%Z
-      end
+  Definition denote (i: instr) p b e a: Z :=
+    match i with
+    | GetP _ _ => encodePerm p
+    | GetB _ _ => b
+    | GetE _ _ => e
+    | GetA _ _ => a
+    | _ => 0%Z
     end.
 
   Global Arguments denote : simpl nomatch.
@@ -58,15 +45,15 @@ Section cap_lang_rules.
     | Get_fail_src_noncap : forall n,
         regs !! src = Some (WInt n) →
         Get_failure i regs dst src
-    | Get_fail_overflow_PC : forall (c:Cap),
-        regs !! src = Some (WCap c) →
-        incrementPC (<[ dst := WInt (denote i c) ]> regs) = None →
+    | Get_fail_overflow_PC : forall p b e a,
+        regs !! src = Some (WCap p b e a) →
+        incrementPC (<[ dst := WInt (denote i p b e a) ]> regs) = None →
         Get_failure i regs dst src.
 
   Inductive Get_spec (i: instr) (regs: Reg) (dst src: RegName) (regs': Reg): cap_lang.val -> Prop :=
-  | Get_spec_success (c: Cap):
-      regs !! src = Some (WCap c) →
-      incrementPC (<[ dst := WInt (denote i c) ]> regs) = Some regs' →
+  | Get_spec_success p b e a:
+      regs !! src = Some (WCap p b e a) →
+      incrementPC (<[ dst := WInt (denote i p b e a) ]> regs) = Some regs' →
       Get_spec i regs dst src regs' NextIV
   | Get_spec_failure:
       Get_failure i regs dst src →
@@ -76,8 +63,8 @@ Section cap_lang_rules.
     decodeInstrW w = get_i →
     is_Get get_i dst src →
 
-    isCorrectPC (WCap (pc_p, pc_b, pc_e, pc_a)) →
-    regs !! PC = Some (WCap (pc_p, pc_b, pc_e, pc_a)) →
+    isCorrectPC (WCap pc_p pc_b pc_e pc_a) →
+    regs !! PC = Some (WCap pc_p pc_b pc_e pc_a) →
     regs_of get_i ⊆ dom _ regs →
     {{{ ▷ pc_a ↦ₐ w ∗
         ▷ [∗ map] k↦y ∈ regs, k ↦ᵣ y }}}
@@ -105,19 +92,19 @@ Section cap_lang_rules.
     erewrite regs_of_is_Get in Hri; eauto.
     destruct (Hri src) as [wsrc [H'src Hsrc]]. by set_solver+.
     destruct (Hri dst) as [wdst [H'dst Hdst]]. by set_solver+.
-    destruct wsrc as [| (([p b] & e) & a) ] eqn:Hwsrc.
+    destruct wsrc as [| p b e a ] eqn:Hwsrc.
     { (* Failure: src is not a capability *)
       assert (c = Failed ∧ σ2 = (r, m)) as (-> & ->).
       { destruct_or! Hinstr; rewrite Hinstr in Hstep; cbn in Hstep.
         all: rewrite /RegLocate Hsrc in Hstep; inversion Hstep; auto. }
       iFailWP "Hφ" Get_fail_src_noncap. }
 
-    assert ((c, σ2) = updatePC (update_reg (r, m) dst (WInt (denote get_i (p,b,e,a))))) as HH.
+    assert ((c, σ2) = updatePC (update_reg (r, m) dst (WInt (denote get_i p b e a)))) as HH.
     { destruct_or! Hinstr; rewrite Hinstr /= in Hstep |- *; auto; cbn in Hstep.
       all: destruct b, e, a; rewrite /RegLocate /update_reg Hsrc /= in Hstep |-*; auto. }
     clear Hstep. rewrite /update_reg /= in HH.
 
-    destruct (incrementPC (<[ dst := WInt (denote get_i (p,  b, e, a)) ]> regs))
+    destruct (incrementPC (<[ dst := WInt (denote get_i p b e a) ]> regs))
       as [regs'|] eqn:Hregs'; pose proof Hregs' as H'regs'; cycle 1.
     { (* Failure: incrementing PC overflows *)
       apply incrementPC_fail_updatePC with (m:=m) in Hregs'.
@@ -142,17 +129,17 @@ Section cap_lang_rules.
   Lemma wp_Get_PC_success E get_i dst pc_p pc_b pc_e pc_a w wdst pc_a' :
     decodeInstrW w = get_i →
     is_Get get_i dst PC →
-    isCorrectPC (WCap (pc_p,pc_b,pc_e,pc_a)) →
+    isCorrectPC (WCap pc_p pc_b pc_e pc_a) →
     (pc_a + 1)%a = Some pc_a' ->
     
-    {{{ ▷ PC ↦ᵣ WCap (pc_p,pc_b,pc_e,pc_a)
+    {{{ ▷ PC ↦ᵣ WCap pc_p pc_b pc_e pc_a
         ∗ ▷ pc_a ↦ₐ w
         ∗ ▷ dst ↦ᵣ wdst }}}
       Instr Executable @ E
       {{{ RET NextIV;
-          PC ↦ᵣ WCap (pc_p,pc_b,pc_e,pc_a')
+          PC ↦ᵣ WCap pc_p pc_b pc_e pc_a'
           ∗ pc_a ↦ₐ w
-          ∗ dst ↦ᵣ WInt (denote get_i (pc_p, pc_b, pc_e, pc_a)) }}}.
+          ∗ dst ↦ᵣ WInt (denote get_i pc_p pc_b pc_e pc_a) }}}.
   Proof.
     iIntros (Hdecode Hinstr Hvpc Hpca' φ) "(>HPC & >Hpc_a & >Hdst) Hφ".
     iDestruct (map_of_regs_2 with "HPC Hdst") as "[Hmap %]".
@@ -169,20 +156,20 @@ Section cap_lang_rules.
       destruct Hfail; try incrementPC_inv; simplify_map_eq; eauto. congruence. }
   Qed.
 
-  Lemma wp_Get_same_success E get_i r pc_p pc_b pc_e pc_a w (c:Cap) pc_a' :
+  Lemma wp_Get_same_success E get_i r pc_p pc_b pc_e pc_a w p' b' e' a' pc_a' :
     decodeInstrW w = get_i →
     is_Get get_i r r →
-    isCorrectPC (WCap (pc_p,pc_b,pc_e,pc_a)) →
+    isCorrectPC (WCap pc_p pc_b pc_e pc_a) →
     (pc_a + 1)%a = Some pc_a' ->
 
-    {{{ ▷ PC ↦ᵣ WCap (pc_p,pc_b,pc_e,pc_a)
+    {{{ ▷ PC ↦ᵣ WCap pc_p pc_b pc_e pc_a
         ∗ ▷ pc_a ↦ₐ w
-        ∗ ▷ r ↦ᵣ WCap c }}}
+        ∗ ▷ r ↦ᵣ WCap p' b' e' a' }}}
       Instr Executable @ E
       {{{ RET NextIV;
-          PC ↦ᵣ WCap (pc_p,pc_b,pc_e,pc_a')
+          PC ↦ᵣ WCap pc_p pc_b pc_e pc_a'
           ∗ pc_a ↦ₐ w
-          ∗ r ↦ᵣ WInt (denote get_i c) }}}.
+          ∗ r ↦ᵣ WInt (denote get_i p' b' e' a') }}}.
   Proof.
     iIntros (Hdecode Hinstr Hvpc Hpca' φ) "(>HPC & >Hpc_a & >Hr) Hφ".
     iDestruct (map_of_regs_2 with "HPC Hr") as "[Hmap %]".
@@ -199,22 +186,22 @@ Section cap_lang_rules.
       destruct Hfail; try incrementPC_inv; simplify_map_eq; eauto. congruence. }
   Qed.
 
-  Lemma wp_Get_success E get_i dst src pc_p pc_b pc_e pc_a w wdst csrc pc_a' :
+  Lemma wp_Get_success E get_i dst src pc_p pc_b pc_e pc_a w wdst p' b' e' a' pc_a' :
     decodeInstrW w = get_i →
     is_Get get_i dst src →
-    isCorrectPC (WCap (pc_p,pc_b,pc_e,pc_a)) →
+    isCorrectPC (WCap pc_p pc_b pc_e pc_a) →
     (pc_a + 1)%a = Some pc_a' ->
 
-    {{{ ▷ PC ↦ᵣ WCap (pc_p,pc_b,pc_e,pc_a)
+    {{{ ▷ PC ↦ᵣ WCap pc_p pc_b pc_e pc_a
         ∗ ▷ pc_a ↦ₐ w
-        ∗ ▷ src ↦ᵣ WCap csrc
+        ∗ ▷ src ↦ᵣ WCap p' b' e' a'
         ∗ ▷ dst ↦ᵣ wdst }}}
       Instr Executable @ E
       {{{ RET NextIV;
-          PC ↦ᵣ WCap (pc_p,pc_b,pc_e,pc_a')
+          PC ↦ᵣ WCap pc_p pc_b pc_e pc_a'
           ∗ pc_a ↦ₐ w
-          ∗ src ↦ᵣ WCap csrc
-          ∗ dst ↦ᵣ WInt (denote get_i csrc) }}}.
+          ∗ src ↦ᵣ WCap p' b' e' a'
+          ∗ dst ↦ᵣ WInt (denote get_i p' b' e' a') }}}.
   Proof.
     iIntros (Hdecode Hinstr Hvpc Hpca' φ) "(>HPC & >Hpc_a & >Hsrc & >Hdst) Hφ".
     iDestruct (map_of_regs_3 with "HPC Hdst Hsrc") as "[Hmap (%&%&%)]".
