theories/examples/counter_adequacy.v
@@ -101,7 +101,7 @@ Definition offset_to_awkward `{memory_layout} : Z :=
 Definition mk_initial_memory `{memory_layout} (adv_val: list Word) : gmap Addr Word :=
   (* pointer to the linking table *)
     list_to_map [(counter_region_start,
-                  WCap (RO, link_table_start, link_table_end, link_table_start))]
+                  WCap RO link_table_start link_table_end link_table_start)]
   ∪ mkregion counter_preamble_start counter_body_start
        (* preamble: code that creates the awkward example closure *)
       (counter_preamble_instrs 0%Z (* offset to malloc in linking table *)
@@ -113,13 +113,13 @@ Definition mk_initial_memory `{memory_layout} (adv_val: list Word) : gmap Addr W
       
   ∪ mkregion adv_start adv_end
       (* adversarial code: any code or data, but no capabilities (see condition below) except for malloc *)
-      (adv_val ++ [WCap (E, malloc_start, malloc_end, malloc_start)])
+      (adv_val ++ [WCap E malloc_start malloc_end malloc_start])
   ∪ mkregion malloc_start malloc_memptr
       (* code for the malloc subroutine *)
       malloc_subroutine_instrs
   ∪ list_to_map
       (* Capability to malloc's memory pool, used by the malloc subroutine *)
-      [(malloc_memptr, WCap (RWX, malloc_memptr, malloc_end, malloc_mem_start))]
+      [(malloc_memptr, WCap RWX malloc_memptr malloc_end malloc_mem_start)]
   ∪ mkregion malloc_mem_start malloc_end
       (* Malloc's memory pool, initialized to zero *)
       (region_addrs_zeroes malloc_mem_start malloc_end)
@@ -127,11 +127,11 @@ Definition mk_initial_memory `{memory_layout} (adv_val: list Word) : gmap Addr W
       ((* code for the failure subroutine *)
         assert_fail_instrs ++
        (* pointer to the "failure" flag, set to 1 by the routine *)
-       [WCap (RW, fail_flag, fail_flag_next, fail_flag)])
+       [WCap RW fail_flag fail_flag_next fail_flag])
   ∪ mkregion link_table_start link_table_end
       (* link table, with pointers to the malloc and failure subroutines *)
-      [WCap (E, malloc_start, malloc_end, malloc_start);
-       WCap (E, fail_start, fail_end, fail_start)]
+      [WCap E malloc_start malloc_end malloc_start;
+       WCap E fail_start fail_end fail_start]
   ∪ list_to_map [(fail_flag, WInt 0%Z)] (* failure flag, initially set to 0 *)
 .
 
@@ -147,8 +147,8 @@ Definition is_initial_memory `{memory_layout} (m: gmap Addr Word) :=
   (adv_start + (length adv_val + 1)%nat)%a = Some adv_end.
 
 Definition is_initial_registers `{memory_layout} (reg: gmap RegName Word) :=
-  reg !! PC = Some (WCap (RX, counter_region_start, counter_region_end, counter_preamble_start)) ∧
-  reg !! r_t0 = Some (WCap (RWX, adv_start, adv_end, adv_start)) ∧
+  reg !! PC = Some (WCap RX counter_region_start counter_region_end counter_preamble_start) ∧
+  reg !! r_t0 = Some (WCap RWX adv_start adv_end adv_start) ∧
   (∀ (r: RegName), r ∉ ({[ PC; r_t0 ]} : gset RegName) →
     ∃ (w:Word), reg !! r = Some w ∧ is_cap w = false).
 
@@ -302,7 +302,7 @@ Section Adequacy.
     iDestruct (big_sepL2_length with "Hadv") as %Hlen2. simpl in Hlen2.
       
     iMod (region_inv_alloc _ (adv_words ++ malloc_word)
-                           (adv_val ++ [WCap (E, malloc_start, malloc_end, malloc_start)])
+                           (adv_val ++ [WCap E malloc_start malloc_end malloc_start])
             with "[Hadv Hmalloc]") as "Hadv".
     { iApply (big_sepL2_app');[auto|]. 
       iSplitL "Hadv". 
@@ -318,7 +318,7 @@ Section Adequacy.
     
     (* Apply the spec, obtain that the PC is in the expression relation *)
 
-    iAssert ((interp_expr interp reg) (WCap (RX, counter_region_start, counter_region_end, counter_preamble_start)))
+    iAssert ((interp_expr interp reg) (WCap RX counter_region_start counter_region_end counter_preamble_start))
       with "[Hcounter_preamble Hcounter_body Hinv_malloc Hcounter_link Hlink1 Hlink2]" as "HE".
     { assert (isCorrectPC_range RX counter_region_start counter_region_end
                                 counter_preamble_start counter_body_start).
