theories/ftlr_binary/Mov_binary.v
@@ -46,7 +46,7 @@ Section fundamental.
     iAssert (⌜w = w'⌝)%I as %Heqw.
     { iDestruct "Hread" as "[Hread _]". iSpecialize ("Hread" with "HP"). by iApply interp_eq. }
     destruct r as [r1 r2]. simpl in *.
-    iDestruct (interp_reg_eq r1 r2 (WCap (p, b, e, a)) with "[]") as %Heq;[iSplit;auto|]. rewrite -!Heq.
+    iDestruct (interp_reg_eq r1 r2 (WCap p b e a) with "[]") as %Heq;[iSplit;auto|]. rewrite -!Heq.
 
     iMod (step_Mov _ [SeqCtx] with "[$Ha' $Hsmap $Hs $Hspec]") as (retv' regs'') "(Hs & #Hmovspec & Ha' & Hsmap) /=";[rewrite Heqw in Hi|..];eauto.
     { rewrite lookup_insert. eauto. }
