theories/logrel_binary.v
@@ -55,7 +55,7 @@ Section logrel.
              ∗ spec_registers_mapsto (<[PC:=w.2]> r.2)
              ∗ na_own logrel_nais ⊤
              ∗ ⤇ Seq (Instr Executable) -∗
-             ⌜match w.1,w.2 with WCap _,WCap _ => True | _,_ => False end⌝ ∧ interp_conf))%I.
+             ⌜match w.1,w.2 with WCap _ _ _ _,WCap _ _ _ _ => True | _,_ => False end⌝ ∧ interp_conf))%I.
   Solve All Obligations with solve_proper.
 
   (* condition definitions *)
@@ -74,7 +74,7 @@ Section logrel.
   Proof. solve_proper. Qed.
 
   Program Definition enter_cond b e a b' e' a' : D -n> iPropO Σ :=
-    λne interp, (∀ r, ▷ □ interp_expr interp r (WCap (RX,b,e,a),WCap (RX,b',e',a')))%I.
+    λne interp, (∀ r, ▷ □ interp_expr interp r (WCap RX b e a, WCap RX b' e' a'))%I.
   Solve Obligations with solve_proper.
   Global Instance enter_cond_ne n :
     Proper ((=) ==> (=) ==> (=) ==> (=) ==> (=) ==> (=) ==> dist n ==> dist n) enter_cond.
@@ -92,14 +92,14 @@ Section logrel.
 
   Program Definition interp_cap_O (interp : D) : D :=
     λne w, (match w with
-            | (WCap (O,b,e,a),WCap (O,b',e',a')) => ⌜b = b' ∧ e = e' ∧ a = a'⌝
+            | (WCap O b e a, WCap O b' e' a') => ⌜b = b' ∧ e = e' ∧ a = a'⌝
             | _ => False
             end)%I.
   Solve All Obligations with solve_proper.
 
   Program Definition interp_cap_RO (interp : D) : D :=
     λne w, (match w with
-            | (WCap (RO,b,e,a),WCap (RO,b',e',a')) =>
+            | (WCap RO b e a, WCap RO b' e' a') =>
               ⌜b = b' ∧ e = e' ∧ a = a'⌝ ∗
               [∗ list] a ∈ (region_addrs b e), ∃ P, inv (logN .@ a) (interp_ref_inv a P) ∗ read_cond P interp
             | _ => False
@@ -108,7 +108,7 @@ Section logrel.
 
   Program Definition interp_cap_RW (interp : D) : D :=
     λne w, (match w with
-            | (WCap (RW,b,e,a),WCap (RW,b',e',a')) =>
+            | (WCap RW b e a, WCap RW b' e' a') =>
               ⌜b = b' ∧ e = e' ∧ a = a'⌝ ∗
                 [∗ list] a ∈ (region_addrs b e), ∃ P, inv (logN .@ a) (interp_ref_inv a P) ∗ read_cond P interp
                                                           ∗ write_cond P interp
@@ -117,7 +117,7 @@ Section logrel.
   Solve All Obligations with solve_proper.
 
   Program Definition interp_cap_RX (interp : D) : D :=
-    λne w, (match w with (WCap (RX,b,e,a),WCap (RX,b',e',a')) =>
+    λne w, (match w with (WCap RX b e a, WCap RX b' e' a') =>
                          ⌜b = b' ∧ e = e' ∧ a = a'⌝ ∗
                          [∗ list] a ∈ (region_addrs b e), ∃ P, inv (logN .@ a) (interp_ref_inv a P) ∗ read_cond P interp
              | _ => False end)%I.
@@ -125,13 +125,13 @@ Section logrel.
 
   Program Definition interp_cap_E (interp : D) : D :=
     λne w, (match w with
-              | (WCap (E,b,e,a),WCap (E,b',e',a')) => ⌜b = b' ∧ e = e' ∧ a = a'⌝ ∗ enter_cond b e a b' e' a' interp
+              | (WCap E b e a, WCap E b' e' a') => ⌜b = b' ∧ e = e' ∧ a = a'⌝ ∗ enter_cond b e a b' e' a' interp
               | _ => False
               end)%I.
   Solve All Obligations with solve_proper.
 
   Program Definition interp_cap_RWX (interp : D) : D :=
-    λne w, (match w with (WCap (RWX,b,e,a),WCap (RWX,b',e',a')) =>
+    λne w, (match w with (WCap RWX b e a, WCap RWX b' e' a') =>
                          ⌜b = b' ∧ e = e' ∧ a = a'⌝ ∗
                            [∗ list] a ∈ (region_addrs b e), ∃ P, inv (logN .@ a) (interp_ref_inv a P) ∗ read_cond P interp
                                                           ∗ write_cond P interp
@@ -143,12 +143,12 @@ Section logrel.
     (λne w,
     match w return _ with
     | (WInt _, WInt _) => interp_z w
-    | (WCap (O, b, e, a),WCap (O, b', e', a')) => interp_cap_O interp w
-    | (WCap (RO, b, e, a),WCap (RO, b', e', a')) => interp_cap_RO interp w
-    | (WCap (RW, b, e, a),WCap (RW, b', e', a')) => interp_cap_RW interp w
-    | (WCap (RX, b, e, a),WCap (RX, b', e', a')) => interp_cap_RX interp w
-    | (WCap (E, b, e, a),WCap (E, b', e', a')) => interp_cap_E interp w
-    | (WCap (RWX, b, e, a),WCap (RWX, b', e', a')) => interp_cap_RWX interp w
+    | (WCap O b e a, WCap O b' e' a') => interp_cap_O interp w
+    | (WCap RO b e a,WCap RO b' e' a') => interp_cap_RO interp w
+    | (WCap RW b e a,WCap RW b' e' a') => interp_cap_RW interp w
+    | (WCap RX b e a,WCap RX b' e' a') => interp_cap_RX interp w
+    | (WCap E b e a,WCap E b' e' a') => interp_cap_E interp w
+    | (WCap RWX b e a,WCap RWX b' e' a') => interp_cap_RWX interp w
     | _ => False
     end)%I.
   Solve All Obligations with solve_proper.
@@ -163,14 +163,14 @@ Section logrel.
     Contractive (interp_cap_RO).
   Proof.
     solve_proper_prepare.
-    destruct x0; auto. destruct o,o0;auto. destruct c, p, p, p,c0,p,p,p; auto.
+    destruct x0; auto. destruct o,o0;auto. destruct p,p0; auto.
     solve_contractive.
   Qed.
   Global Instance interp_cap_RW_contractive :
     Contractive (interp_cap_RW).
   Proof.
     solve_proper_prepare.
-    destruct x0; auto. destruct o,o0;auto. destruct c, p, p, p,c0,p,p,p; auto.
+    destruct x0; auto. destruct o,o0;auto. destruct p,p0; auto.
     solve_contractive.
   Qed.
   Global Instance enter_cond_contractive b e a b' e' a'  :
@@ -182,21 +182,21 @@ Section logrel.
     Contractive (interp_cap_RX).
   Proof.
     solve_proper_prepare.
-    destruct x0; auto. destruct o,o0;auto. destruct c, p, p, p,c0,p,p,p; auto.
+    destruct x0; auto. destruct o,o0;auto. destruct p,p0; auto.
     solve_contractive.
   Qed.
   Global Instance interp_cap_E_contractive :
     Contractive (interp_cap_E).
   Proof.
     solve_proper_prepare.
-    destruct x0; auto. destruct o,o0;auto. destruct c, p, p, p,c0,p,p,p; auto.
+    destruct x0; auto. destruct o,o0;auto. destruct p,p0; auto.
     solve_contractive.
   Qed.
   Global Instance interp_cap_RWX_contractive :
     Contractive (interp_cap_RWX).
   Proof.
     solve_proper_prepare.
-    destruct x0; auto. destruct o,o0;auto. destruct c, p, p, p,c0,p,p,p; auto.
+    destruct x0; auto. destruct o,o0;auto. destruct p,p0; auto.
     solve_contractive.
   Qed.
 
@@ -207,7 +207,7 @@ Section logrel.
     intros n x y Hdistn [w w0].
     rewrite /interp1.
     destruct w,w0; [auto..|].
-    destruct c,p,p,p,c0,p,p,p; try auto.
+    destruct p,p0; try auto.
     - by apply interp_cap_RO_contractive.
     - by apply interp_cap_RW_contractive.
     - by apply interp_cap_RX_contractive.
@@ -225,13 +225,13 @@ Section logrel.
 
   Global Instance interp_persistent w : Persistent (interp w).
   Proof. intros. destruct w as [w w0]. destruct w,w0; simpl; rewrite fixpoint_interp1_eq; simpl;
-         try destruct c,p,p,p;try apply _;destruct c0,p,p,p; repeat (apply exist_persistent; intros); try apply _.
+         try destruct p;try apply _;destruct p0; repeat (apply exist_persistent; intros); try apply _.
   Qed.
 
   Lemma read_allowed_inv (a'' a b e a' b' e' : Addr) p p' :
     (b ≤ a'' ∧ a'' < e)%Z →
     readAllowed p →
-    ⊢ (interp (WCap (p,b,e,a),WCap (p',b',e',a')) →
+    ⊢ (interp (WCap p b e a,WCap p' b' e' a') →
      (∃ P, inv (logN .@ a'') (interp_ref_inv a'' P) ∗ read_cond P interp ∗ if writeAllowed p then write_cond P interp else emp))%I.
   Proof.
     iIntros (Hin Ra) "Hinterp".
@@ -244,7 +244,7 @@ Section logrel.
   Lemma write_allowed_inv (a'' a b e a' b' e' : Addr) p p' :
     (b ≤ a'' ∧ a'' < e)%Z →
     writeAllowed p →
-    ⊢ (interp (WCap (p,b,e,a), WCap (p',b',e',a')) →
+    ⊢ (interp (WCap p b e a, WCap p' b' e' a') →
      inv (logN .@ a'') (interp_ref_inv a'' interp))%I.
   Proof.
     iIntros (Hin Wa) "Hinterp".
@@ -275,8 +275,8 @@ Section logrel.
     (b ≤ a'' ∧ a'' < e)%Z →
     readAllowed p →
     ⊢ (interp_registers r -∗
-    interp (WCap (p,b,e,a),WCap (p',b',e',a')) -∗
-     (∃ P, inv (logN .@ a'') (interp_ref_inv a'' P) ∗ read_cond P interp ∗ if decide (writeAllowed_in_r_a (<[PC:=WCap (p,b,e,a)]> r.1) a'') then write_cond P interp else emp))%I.
+    interp (WCap p b e a,WCap p' b' e' a') -∗
+     (∃ P, inv (logN .@ a'') (interp_ref_inv a'' P) ∗ read_cond P interp ∗ if decide (writeAllowed_in_r_a (<[PC:=WCap p b e a]> r.1) a'') then write_cond P interp else emp))%I.
   Proof.
     iIntros (Hin Ra) "#Hregs #Hinterp".
     rewrite /interp_registers /interp_reg /=.
@@ -294,11 +294,11 @@ Section logrel.
       + rewrite /RegLocate in Hwa Ha. rewrite lookup_insert_ne// in Hwa,Ha.
         destruct (r.1 !! reg) eqn:Hsome;rewrite Hsome in Ha Hwa; [|inversion Ha].
         assert (is_Some(r.2 !! reg)) as [? ?];[by destruct H0 with reg|].
-        destruct w;[inversion Ha|]. destruct c,p0,p0. destruct Ha as [Hwba ->].
+        destruct w;[inversion Ha|]. destruct Ha as [Hwba ->].
         iSpecialize ("Hregvalid" $! _ n). rewrite /RegLocate Hsome H1. iClear "Hinterp".
         rewrite /interp. cbn. rewrite fixpoint_interp1_eq /=; cbn.
-        destruct x; [destruct p0;done|].
-        destruct p0,p',c,p0,p0,p0; try contradiction; try done; inversion Hwa;
+        destruct x; [destruct p0; done |].
+        destruct p0,p1; try contradiction; try done; inversion Hwa;
         try (iDestruct "Hregvalid" as "[(%&%&%) Hregvalid]";simplify_eq);
         try (iDestruct (extract_from_region_inv with "Hregvalid") as (P) "[Hinv Hiff]"; [eauto|iExists P;iSplit;eauto]).
     - rewrite /interp. cbn. rewrite fixpoint_interp1_eq /=; cbn.
@@ -332,8 +332,8 @@ Section logrel.
   Proof.
     iIntros "Hv".
     rewrite fixpoint_interp1_eq /=.
-    destruct w,w';try done. by iDestruct "Hv" as %->. destruct c,p,p,p;done.
-    destruct c,p,p,p,c0,p,p,p;try done;[by iDestruct "Hv" as %(->&->&->)|by iDestruct "Hv" as "[Hv _]"; iDestruct "Hv" as %(->&->&->)..].
+    destruct w,w';try done. by iDestruct "Hv" as %->. destruct p;done.
+    destruct p,p0;try done;[by iDestruct "Hv" as %(->&->&->)|by iDestruct "Hv" as "[Hv _]"; iDestruct "Hv" as %(->&->&->)..].
   Qed.
 
   Lemma interp_reg_eq (r r' : Reg) (w : Word) :
